fixes

Test/civl/inductive-sequentialization/snapshot-scatter-gather-full.bpl
@@ -13,20 +13,6 @@ datatype Permission {
     Permission(t_id: Tid, mem_index: int)
 }
 
-// permissions need to put back in globals to retry later
-// how to know scan ended
-// if r1 == r2, return snapshot 
-
-
-// implement one iteration
-// first scan, second scan 
-// if it succeeds then good, otherwise nothing.
-
-
-
-// prove that snapshot is correct if it succeeds.
-// make it retryable anyway
-
 const n: int;
 axiom n >= 1;
 
@@ -39,62 +25,53 @@ function {:inline} WholeTidPermission(tid: Tid): Set Permission {
   Set((lambda {:pool "TidPermission"} x: Permission :: x->t_id == tid && (1 <= x->mem_index) && (x->mem_index <= n)))
 }
 
-action {:layer 1} start ({:linear_in} tid: One Tid)
+action {:layer 1} start (tid: Tid)
 modifies pSet;
 creates main_f;
 {
     var {:linear} sps: Set Permission;
-    call sps := Set_Get(pSet, (lambda x: Permission :: (x->t_id == tid->val) && (1 <= x->mem_index) && (x->mem_index <= n)));
+    call sps := Set_Get(pSet, (lambda x: Permission :: (x->t_id == tid) && (1 <= x->mem_index) && (x->mem_index <= n)));
     call create_async(main_f(tid, sps));
 }
 
 // M =  main_f , \elim = read_f, I = Inv_f, M' = main_f'
-async action {:layer 1} main_f({:linear_in} tid: One Tid, {:linear} sps: Set Permission)
+async action {:layer 1} main_f(tid: Tid, {:linear_in} sps: Set Permission)
 refines {:IS_right} main_f' using Inv_f;
 modifies pSet;
 creates read_f;
 {
     // var {:linear} sps: Set Permission;
     // assume {:add_to_pool "A", 0} true;
-    call create_asyncs((lambda pa:read_f :: (1 <= pa->i) && (pa->i <= n) && pa->perm == One(Permission(tid->val, pa->i))));
+    // assert (sps == Set((lambda x: Permission :: (x->t_id == tid) && (1 <= x->mem_index) && (x->mem_index <= n))));
+    call create_asyncs((lambda pa:read_f :: (1 <= pa->i) && (pa->i <= n) && pa->perm == One(Permission(tid, pa->i))));
 }
 
-async action {:layer 1, 2} gather_f()
-// modifies pSet;
-{
-    // call One_Put(pSet, perm);
-    // // call Set_Get(pSet(lambda x: Permission :: (x->t_id == tid->val) && (1 <= x->mem_index) && (x->mem_index <= n)));
-    // // if (*){
-    // assume Set_IsSubset(WholeTidPermission(tid->val), pSet);
-    // // }
-}
 
-action {:layer 2} main_f'({:linear_in} tid: One Tid, {:linear} sps: Set Permission)
-creates gather_f;
+
+action {:layer 2} main_f'(tid: Tid, {:linear_in} sps: Set Permission)
+creates main_s;
 modifies r1, pSet;
 {
-    // var {:linear} sps: Set Permission;
+    var {:linear} sps2: Set Permission;
     var {:linear} done_set: Set Permission;
-
-    // call sps := Set_Get(pSet, (lambda x: Permission :: (x->t_id == tid->val) && (1 <= x->mem_index) && (x->mem_index <= n)));
+    sps2 := sps;
+    // call sps := Set_Get(pSet, (lambda x: Permission :: (x->t_id == tid) && (1 <= x->mem_index) && (x->mem_index <= n)));
+    assume (sps == Set((lambda x: Permission :: (x->t_id == tid) && (1 <= x->mem_index) && (x->mem_index <= n))));
     havoc r1;
-    assume (forall i:int :: ((1 <= i && i <= n) ==> (r1[tid->val][i]->ts < mem[i]->ts  || r1[tid->val][i]== mem[i]))); 
-    // call done_set := Set_Get(sps, (lambda x: Permission :: (x->t_id == tid->val) && (1 <= x->mem_index) && (x->mem_index <= n))); 
-    // call Set_Put(pSet, done_set);
-    call create_async(gather_f());
+    assume (forall i:int :: ((1 <= i && i <= n) ==> (r1[tid][i]->ts < mem[i]->ts  || r1[tid][i]== mem[i]))); 
+    call done_set := Set_Get(sps2, (lambda x: Permission :: (x->t_id == tid) && (1 <= x->mem_index) && (x->mem_index <= n))); 
+    call Set_Put(pSet, done_set);
+    call create_async(main_s(tid));
 
 }
 
 async action {:layer 1} read_f({:linear_in} perm: One Permission, i: int)
-creates read_f, gather_f;
+creates read_f, main_s;
 modifies r1, pSet;
-// requires {:layer 1} Set_IsSubset(WholeTidPermission(perm->val->t_id), old(pSet));
-// call YieldPing(x, p);
-// {:exit} 
 {
     var {:pool "K"} k:int;
     var {:pool "V"} v:Value;
-    assume {:exit_condition Set_IsSubset(WholeTidPermission(perm->val->t_id), old(pSet))} true;
+    assume {:exit_condition Set_IsSubset(WholeTidPermission(perm->val->t_id), pSet)} true;
 
     if (*) {
         assume {:add_to_pool "K", mem[i]->ts, k} {:add_to_pool "V", mem[i]->value, v} true;
@@ -106,47 +83,10 @@ modifies r1, pSet;
     call One_Put(pSet, perm);
 
     if (Set_IsSubset(WholeTidPermission(perm->val->t_id), pSet)){
-        // call create_async(main_s(perm->val->t_id));
-        call create_async(gather_f());
+        call create_async(main_s(perm->val->t_id));
     }
 }
 
-
-// We check for exit that: 
-// 1. assume exit, call A, any pa created is not in \elim  or no pa is created
-// 2. assume not exit, call A, any pa created is in \elim or no pa is created
-// Inconsistency check: forall E1, E2: (E1 and E2 are descendants of M) => gate(E1) and (gate(E2)+exit) can't be true together
-
-
-
-
-// check 1: assume beta, any pa is in \elim or creates no pas
-// check 2: assume not beta, any pa is not in \elim or create no pas
-// beta = true as default (whole action is a right mover)
-
-// chi = not beta (maybe)
-
-// inconsistency: normal action execution , not beta action execution should be inconsistent together.
-
-
-//specify negation : specify the exit (chi)
-
-async action {:layer 1} alpha_read_f({:linear_in} perm: One Permission, i: int)
-creates read_f;
-modifies r1, pSet;
-{
-    var {:pool "K"} k:int;
-    var {:pool "V"} v:Value;
-
-    if (*) {
-        assume {:add_to_pool "K", mem[i]->ts, k} {:add_to_pool "V", mem[i]->value, v} true;
-        assume k < mem[i]->ts; 
-        r1[perm->val->t_id][i]:= StampedValue(k, v);
-    } else {
-        r1[perm->val->t_id][i]:= mem[i];
-    }
-    call One_Put(pSet, perm);
-}
 
 atomic action {: layer 1,2} write(i: int,v: Value)
 modifies mem;
@@ -157,54 +97,52 @@ modifies mem;
     mem[i] := StampedValue(x->ts + 1, v);
 }
 
-action {:layer 1} Inv_f({:linear_in} tid: One Tid, {:linear} sps: Set Permission)
+action {:layer 1} Inv_f(tid: Tid, {:linear_in} sps: Set Permission)
 modifies r1, pSet;
-creates read_f, gather_f;
+creates read_f, main_s;
 {
     var {:pool "A"} j: int;
-    // var {:linear} sps: Set Permission;
+    var {:linear} sps2: Set Permission;
     var {:linear} done_set: Set Permission;
     var choice: read_f;
-
-    // call sps := Set_Get(pSet, (lambda x: Permission :: (x->t_id == tid->val) && (1 <= x->mem_index) && (x->mem_index <= n)));
+    sps2 := sps;
+    // call sps := Set_Get(pSet, Set(lambda x: Permission :: (x->t_id == tid) && (1 <= x->mem_index) && (x->mem_index <= n)));
+    assume sps == Set((lambda x: Permission :: (x->t_id == tid) && (1 <= x->mem_index) && (x->mem_index <= n)));
     assume {:add_to_pool "A", j+1, 0} 0 <= j && j <= n;
     havoc r1;
-    assume (forall i:int :: ((1 <= i && i <= j) ==> (r1[tid->val][i]->ts < mem[i]->ts || r1[tid->val][i]== mem[i]))); 
-    // call done_set := Set_Get(sps, (lambda x: Permission :: (x->t_id == tid->val) && (1 <= x->mem_index) && (x->mem_index <= j))); 
-    // call Set_Put(pSet, sps);
+    assume (forall i:int :: ((1 <= i && i <= j) ==> (r1[tid][i]->ts < mem[i]->ts || r1[tid][i]== mem[i]))); 
+    call done_set := Set_Get(sps2, (lambda x: Permission :: (x->t_id == tid) && (1 <= x->mem_index) && (x->mem_index <= j))); 
+    call Set_Put(pSet, sps2);
     if (j < n){
-        choice := read_f(One(Permission(tid->val, j+1)), j+1);
+        choice := read_f(One(Permission(tid, j+1)), j+1);
         assume {:add_to_pool "C", choice} true;
-        call create_asyncs((lambda {:pool "C" } pa:read_f :: ((j+1) <= pa->i) && (pa->i <= n) && pa->perm == One(Permission(tid->val, pa->i))));
+        call create_asyncs((lambda {:pool "C" } pa:read_f :: ((j+1) <= pa->i) && (pa->i <= n) && pa->perm == One(Permission(tid, pa->i))));
         call set_choice(choice);
     }
 }
 
 // // ISL part
-
-
-
 // M =  main_s , \elim = read_s, I = Inv_s, M' = main_s'
-// async action {:layer 1} main_s({:linear_in} tid: One Tid)
+async action {:layer 1,2} main_s(tid: Tid)
 // refines {:IS_left} main_s' using Inv_s;
 // modifies pSet;
 // creates read_s;
-// {
-//     var {:linear} sps: Set Permission;
+{
+    // var {:linear} sps: Set Permission;
 
-//     assume {:add_to_pool "A", 0} true;
-//     call sps := Set_Get(pSet, (lambda x: Permission :: (x->t_id == tid->val) && (1 <= x->mem_index) && (x->mem_index <= n)));
-//     call create_asyncs((lambda pa:read_s :: (1 <= pa->i) && (pa->i <= n) && pa->perm == One(Permission(tid->val, pa->i))));
-// }
+    // assume {:add_to_pool "A", 0} true;
+    // call sps := Set_Get(pSet, (lambda x: Permission :: (x->t_id == tid) && (1 <= x->mem_index) && (x->mem_index <= n)));
+    // call create_asyncs((lambda pa:read_s :: (1 <= pa->i) && (pa->i <= n) && pa->perm == One(Permission(tid, pa->i))));
+}
 
 // action {:layer 2} main_s'({:linear_in} tid: One Tid)
 // modifies r2, pSet;
 // {
 //     var {:linear} sps: Set Permission;
 
-//     call sps := Set_Get(pSet, (lambda x: Permission :: (x->t_id == tid->val) && (1 <= x->mem_index) && (x->mem_index <= n)));
+//     call sps := Set_Get(pSet, (lambda x: Permission :: (x->t_id == tid) && (1 <= x->mem_index) && (x->mem_index <= n)));
 //     havoc r2;
-//     assume (forall i:int :: ((1 <= i && i <= n) ==> (r2[tid->val][i]->ts > mem[i]->ts  || r2[tid->val][i] == mem[i]))); 
+//     assume (forall i:int :: ((1 <= i && i <= n) ==> (r2[tid][i]->ts > mem[i]->ts  || r2[tid][i] == mem[i]))); 
 // }
 
 // async action {:layer 1} read_s({:linear_in} perm: One Permission, i: int)
@@ -231,14 +169,59 @@ creates read_f, gather_f;
 //     var {:linear} sps: Set Permission;
 //     var choice: read_s;
 
-//     call sps := Set_Get(pSet, (lambda x: Permission :: (x->t_id == tid->val) && (1 <= x->mem_index) && (x->mem_index <= n)));
+//     call sps := Set_Get(pSet, (lambda x: Permission :: (x->t_id == tid) && (1 <= x->mem_index) && (x->mem_index <= n)));
 //     assume {:add_to_pool "A", j+1} 0 <= j && j <= n;
 //     havoc r2;
-//     assume (forall i:int :: ((1 <= i && i <= j) ==> (r2[tid->val][i]->ts > mem[i]->ts || r2[tid->val][i] == mem[i]))); 
+//     assume (forall i:int :: ((1 <= i && i <= j) ==> (r2[tid][i]->ts > mem[i]->ts || r2[tid][i] == mem[i]))); 
 //     if (j < n){
-//         choice := read_s(One(Permission(tid->val, j+1)), j+1);
+//         choice := read_s(One(Permission(tid, j+1)), j+1);
 //         assume {:add_to_pool "C", choice} true;
-//         call create_asyncs((lambda {:pool "C" } pa:read_s :: ((j+1) <= pa->i) && (pa->i <= n) && pa->perm == One(Permission(tid->val, pa->i))));
+//         call create_asyncs((lambda {:pool "C" } pa:read_s :: ((j+1) <= pa->i) && (pa->i <= n) && pa->perm == One(Permission(tid, pa->i))));
 //         call set_choice(choice);
 //     }
+// }
+
+// permissions need to put back in globals to retry later
+// how to know scan ended
+// if r1 == r2, return snapshot 
+
+
+// implement one iteration
+// first scan, second scan 
+// if it succeeds then good, otherwise nothing.
+
+
+
+// prove that snapshot is correct if it succeeds.
+// make it retryable anyway
+
+
+
+// We check for exit that: 
+// 1. assume exit, call A, any pa created is not in \elim  or no pa is created
+// 2. assume not exit, call A, any pa created is in \elim or no pa is created
+// Inconsistency check: forall E1, E2: (E1 and E2 are descendants of M) => gate(E1) and (gate(E2)+exit) can't be true together
+
+
+
+
+// check 1: assume beta, any pa is in \elim or creates no pas
+// check 2: assume not beta, any pa is not in \elim or create no pas
+// beta = true as default (whole action is a right mover)
+
+// chi = not beta (maybe)
+
+// inconsistency: normal action execution , not beta action execution should be inconsistent together.
+
+
+//specify negation : specify the exit (chi)
+
+// async action {:layer 1, 2} gather_f()
+// // modifies pSet;
+// {
+//     // call One_Put(pSet, perm);
+//     // // call Set_Get(pSet(lambda x: Permission :: (x->t_id == tid) && (1 <= x->mem_index) && (x->mem_index <= n)));
+//     // // if (*){
+//     // assume Set_IsSubset(WholeTidPermission(tid), pSet);
+//     // // }
 // }
